src/CoindIndexed.v
@@ -1,0 +1,70 @@
+From Coq Require Import List.
+Import List.ListNotations.
+Open Scope list_scope.
+From Coq Require Import Setoid.
+From Coq Require Import Morphisms.
+From Coq Require Import NPeano.
+From Coq Require Import Omega.
+From Coq Require Import Program.Tactics.
+
+From Velus Require Import Common.
+From Velus Require Import Environment.
+From Velus Require Import Operators.
+From Velus Require Import IndexedStreams.
+From Velus Require Import CoindStreams.
+From Velus Require Import CoindToIndexed IndexedToCoind.
+
+Module Type COINDINDEXED
+       (Import Op    : OPERATORS)
+       (Import OpAux : OPERATORS_AUX Op)
+       (Import CStr  : COINDSTREAMS Op OpAux)
+       (Import IStr  : INDEXEDSTREAMS Op OpAux).
+
+  Module Export CIStr := CoindToIndexedFun Op OpAux CStr IStr.
+  Module Export ICStr := IndexedToCoindFun Op OpAux IStr CStr.
+
+  Fact tr_stream_eqst {A} : forall (x : Stream A),
+      ICStr.tr_stream (tr_Stream x) ≡ x.
+  Proof.
+    unfold ICStr.tr_stream, ICStr.tr_stream_from, tr_Stream.
+    intros x.
+    apply ntheq_eqst; intros n.
+    rewrite ICStr.init_from_nth, Nat.add_0_r.
+    reflexivity.
+  Qed.
+
+  Fact tr_history_equiv: forall H,
+      Env.Equiv (@EqSt value) (ICStr.tr_history (CIStr.tr_history H)) H.
+  Proof.
+    intros H.
+    unfold CIStr.tr_history, ICStr.tr_history, ICStr.tr_history_from.
+    constructor; intros.
+    - rewrite Env.Props.P.F.mapi_in_iff, Env.Props.P.F.map_in_iff. reflexivity.
+    - unfold Env.MapsTo in H0. rewrite Env.gmapi in H0.
+      apply option_map_inv_Some in H0 as [v [Hfind Hinit]]; subst.
+      apply ntheq_eqst. intros n.
+      rewrite ICStr.init_from_nth, Nat.add_0_r, Env.Props.P.F.map_o, H1; simpl; auto.
+  Qed.
+
+  Lemma sem_clock_equiv : forall H b ck bs,
+      CStr.sem_clock H b ck bs <->
+      IStr.sem_clock (tr_Stream b) (CIStr.tr_history H) ck (tr_Stream bs).
+  Proof.
+    intros; split.
+    - apply CIStr.sem_clock_impl.
+    - intro Hsem.
+      apply ICStr.sem_clock_impl in Hsem.
+      repeat rewrite tr_stream_eqst in Hsem. rewrite tr_history_equiv in Hsem.
+      assumption.
+  Qed.
+
+End COINDINDEXED.
+
+Module CoindIndexedFun
+       (Op      : OPERATORS)
+       (OpAux   : OPERATORS_AUX          Op)
+       (CStr    : COINDSTREAMS           Op OpAux)
+       (IStr    : INDEXEDSTREAMS         Op OpAux)
+<: COINDINDEXED Op OpAux CStr IStr.
+  Include COINDINDEXED Op OpAux CStr IStr.
+End CoindIndexedFun.
